Fix validator definition and correctness
A validator is a special case of a parser (one that returns a unit), so
re-use the definition. This also inherits the and_then combinator.

There was a bug in the correctness specification that actually made
`validate_many` incorrect: the validator must also consume the same
number of bytes as the parser, otherwise the composition of validators
doesn't work for the composition of parsers as their positions in the
input buffer might become desynchronized.

examples/struct/keyvalue.pos/Test.fst
@@ -220,37 +220,36 @@ let encode s = u32_to_be s.num_entries `append`
 
 (*! Validating input buffer *)
 
-(** like a parser, a validator returns the number of bytes consumed *)
-let validator = b:bytes -> bool * n:nat{n <= length b}
+let validator = parser unit
 // let parse_validator #t (p:parser t) = b:bytes -> (ok:bool{ok <==> Some? (p b)} * n:nat{n <= length b})
 
-val seq_check: validator -> validator -> validator
-let seq_check v1 v2 b =
-  let (ok, l) = v1 b in
-  if ok = false then (false, l)
-  else
-  let (ok, l') = v2 (slice b l (length b)) in
-  (ok, l + l')
+unfold let seq (#t:Type) (#t':Type) (p:parser t) (p': parser t') : parser t' =
+  fun b -> match p b with
+        | Some (_, l) -> begin
+            match p' (slice b l (length b)) with
+            | Some (v, l') -> Some (v, l + l')
+            | None -> None
+          end
+        | None -> None
 
-val then_validate : #t:Type -> parser t -> (t -> validator) -> validator
-let then_validate #t p v b =
-  match p b with
-  | Some (r, l) -> begin
-      let (ok, l') = v r (slice b l (length b)) in
-      (ok, l + l')
-    end
-  | None -> (false, 0)
+let invalid (#b:bytes): option (unit * n:nat{n <= length b}) = None
+let valid (#b:bytes) (n:nat{n <= length b}) : option (unit * n:nat{n <= length b}) = Some ((), n)
 
 let skip_bytes (n:nat) : validator =
-  fun b -> if length b < n then (false, length b)
-        else (true, n)
+  fun b -> if length b < n then invalid
+        else valid n
 
 // NOTE: this proof about the whole validator works better than a function with
 // built-in correctness proof (despite the universal quantifier)
 (** a correctness condition for a validator, stating that it correctly reports
    when a parser will succeed (the implication only needs to be validated ==>
    will parse, but this has worked so far) *)
-let validator_checks (v:validator) #t (p: parser t) = forall b. fst (v b) == true <==> Some? (p b)
+unfold let validator_checks (v:validator) #t (p: parser t) = forall b. Some? (v b) ==> (Some? (p b) /\ snd (Some?.v (v b)) == snd (Some?.v (p b)))
+
+// this definitions assists type inference by forcing t'=unit; it also makes the
+// code read a bit better
+unfold let then_validate (#t:Type) (p:parser t) (v:t -> validator) : validator =
+    and_then p v
 
 val validate_u16_array: v:validator{validator_checks v parse_u16_array}
 let validate_u16_array =
@@ -263,13 +262,13 @@ let validate_u32_array =
   (fun array_len -> skip_bytes (U32.v array_len))
 
 let validate_entry: v:validator{validator_checks v parse_entry} =
-  validate_u16_array `seq_check`
+  validate_u16_array `seq`
   validate_u32_array
 
 let validate_accept : validator =
-  fun b -> (true, 0)
+  fun b -> valid 0
 let validate_reject : validator =
-  fun b -> (false, 0)
+  fun b -> invalid
 
 val validate_many':
   n:nat ->
@@ -278,14 +277,33 @@ val validate_many':
 let rec validate_many' n v =
   match n with
   | 0 -> validate_accept
-  | _ -> v `seq_check` validate_many' (n-1) v `seq_check` validate_accept
+  | _ -> v `seq` validate_many' (n-1) v
 
-let rec validate_many'_ok (n:nat) (#t:Type) (p: parser t) (v:validator) :
-  Lemma (requires (validator_checks v p))
+let validate_seq (#t:Type) (#t':Type)
+  (p: parser t) (p': parser t')
+  (v: validator{validator_checks v p})
+  (v': validator{validator_checks v' p'}) :
+  Lemma (validator_checks (v `seq` v') (p `seq` p')) = ()
+
+let validate_liftA2 (#t:Type) (#t':Type) (#t'':Type)
+  (p: parser t) (p': parser t') (f: t -> t' -> t'')
+  (v: validator{validator_checks v p})
+  (v': validator{validator_checks v' p'}) :
+  Lemma (validator_checks (v `seq` v') (p `and_then` (fun (x:t) -> p' `and_then` (fun (y:t') -> parse_ret (f x y))))) =
+  assert (forall x. validator_checks v' (p' `and_then` (fun y -> parse_ret (f x y))));
+  ()
+
+// #set-options "--z3rlimit 10"
+
+let rec validate_many'_ok (n:nat) (#t:Type) (p: parser t) (v:validator{validator_checks v p}) :
+  Lemma (requires True)
         (ensures (validator_checks (validate_many' n v) (parse_many' p n))) =
   match n with
   | 0 -> ()
-  | _ -> admit(); validate_many'_ok (n-1) p v
+  | _ -> validate_many'_ok (n-1) p v;
+        let p' = parse_many' p (n-1) in
+        validate_liftA2 p p' (fun v l -> v::l) v (validate_many' (n-1) v <: (v:validator{validator_checks v p'}));
+        ()
 
 val validate_many:
   #t:Type -> p:parser t ->
@@ -295,15 +313,15 @@ val validate_many:
 let validate_many #t p n v = validate_many'_ok n p v; validate_many' n v
 
 let validate_done : v:validator{validator_checks v parsing_done} =
-  fun b -> if length b = 0 then (true, 0)
-        else (false, 0)
+  fun b -> if length b = 0 then valid 0
+        else invalid
 
 val validate: v:validator{validator_checks v parse_abstract_store}
 let validate =
   admit();
   parse_u32 `then_validate`
-  (fun num_entries -> validate_many parse_entry (U32.v num_entries) validate_entry `seq_check`
-                   validate_done `seq_check`
+  (fun num_entries -> validate_many parse_entry (U32.v num_entries) validate_entry `seq`
+                   validate_done `seq`
                    validate_accept)
 
 (*! API using validated but unparsed key-value buffer *)
@@ -335,11 +353,8 @@ let parse_value_offset (b:bytes) : option (n:nat{n <= length b}) =
     // length (so that b is parseable as an entry); the slice of the remaining
     // input should become part of the parser incrementing a current position
     // pointer into the input buffer
-    match validate_u32_array (slice b l (length b)) with
-    | (true, _) -> Some l
-    | (false, _) -> None)
-
-#reset-options "--z3rlimit 10"
+    validate_u32_array (slice b l (length b)) `optbind`
+    (fun _ -> Some l))
 
 let parse_value_offset_ok (b:bytes) :
   Lemma (parse_value_offset b `optbind`
